src/Equiv.v
@@ -1,0 +1,16 @@
+Class Equiv A :=
+  { equiv : A -> A -> Prop }.
+
+Definition eq_equiv {A B} (f : A -> B) (a1 a2 : A) :=
+  f a1 = f a2.
+
+Infix "===" := equiv (at level 70, no associativity).
+
+Global Instance EquivPair0 {A B} `{Equiv A} `{Equiv B} : Equiv (A * B) | 0 :=
+  { equiv x y := fst x === fst y /\ snd x === snd y }.
+
+Global Instance EquivPair1 {A B} `{Equiv A} : Equiv (A * B) | 1 :=
+  { equiv x y := fst x === fst y /\ snd x = snd y }.
+
+Global Instance EquivPair2 {A B} `{Equiv B} : Equiv (A * B) | 1 :=
+  { equiv x y := fst x = fst y /\ snd x === snd y }.
